\documentclass{article}
\usepackage[T1]{fontenc}
\usepackage[utf8]{inputenc}
\usepackage{unicode,math}
\usepackage[margin=30mm]{geometry}
\newenvironment{eqsplit}{\equation\aligned}{\endaligned\endequation}


\begin{document}
\title{Useful geometric computatoins}


\section{Uniform approximation of a parabolic arc by a polygonal chain}%Â«Â«1
\begin{prop}\label{prop:points}
Let~$ğ’«$ be the parabola with equation $y = f(x) = a/2 + xÂ²/2a$.
Let~$H$ be the hypergeometric function
$H(u) = {}_2F_1(1/4,1/2;\;3/2\;-u^2)$.

Choose real numbers~$s_1$, $s_2$ and an integer~$n â‰¥ 1$
and define, for~$i = 0, â€¦, n$,
$x_i = a H^{-1}((1-i/n) s_1 + (i/n) s_2)$.

Then, for $n$ large enough,
the polygonal line with vertices~$A_i = (x_i, f(x_i))$
lies within a Minkowski distance~$Î´ = \frac{a}{8n^2}
(s_2-s_1)^2+O(n^{-4})$ of the parabola~$ğ’«$.
\end{prop}

\begin{proof}
It is enough to prove this for an individual segment of the polygonal line,
for example the segment $(A_0, A_1)$.
For~$x_0 â‰¤ x â‰¤ x_1$, the distance between a point~$(x, f(x)) âˆˆ ğ’«$
and the segment~$(A_0, A_1)$ is given by the function
% 	the maximum on the interval~$[x_0,x_1]$ of the function
\begin{equation}\begin{split}
g(x)
%  &= \frac{(x_0+x_1)/(2a) x - f(x) + x_0 x_1/(2a) + a/2}{âˆš{1+(x_0+x_1/2a)^2}}\\
 &= \frac{(x_0+x_1) x - 2a f(x) + x_0 x_1 + a^2}{âˆš{(2a)^2+(x_0+x_1)^2}}\\
%  &= \frac{(x_0+x_1) x - a^2 - x^2 + x_0 x_1 + a^2}{âˆš{(2a)^2+(x_0+x_1)^2}}\\
 &= \frac{(x-x_0)(x_1-x)}{âˆš{(2a)^2+(x_0+x_1)^2}}.\\
\end{split}\end{equation}
The maximum value~$Î´_0$ of~$g$ on the interval~$[x_0,x_1]$
is reached for~$x = (x_0+x_1)/2$
and amounts to $Î´_0 = \frac{(x_1-x_0)^2}{4âˆš{(2a)^2+(x_0+x_1)^2}}$.

Let~$G = H^{-1}$ and~$x(t) = a G((1-t) s_1 + t s_2)$.
Then for all~$i = 0,â€¦, n$, $x_i = x(i/n)$
and $x_{i+1} - x_i = x'(i/n)/n + O(1/n^2)$.
Therefore
\begin{equation}
Î´_i = \frac{x'(i/n)^2}{8n^2 âˆš{a^2 + x_i^2}} + O(1/n^4).
\end{equation}

Since $H'(u)^4 = 1/(1+u^2)$,
the inverse~$G$ of~$H$ satisfies the differential equation
$(G')^4 = 1 + G^2$,
and hence $x'(t)^2 = a (s_2 - s_1)^2 âˆš{a^2 + x(t)^2}$.
Accordingly, one finds
\begin{equation}
Î´_i = \frac{a}{8n^2} (s_2-s_1)^2 + O(1/n^4).
\end{equation}
Since this is true for all~$i = 0,â€¦,n-1$, the proposition follows.
\end{proof}


\begin{prop}\label{prop:approx}
The following algorithm approximates the parabola~$ğ’«$
on the interval~$[X_1,X_2]$ within a distance~$â‰¤ Î´ + O(Î´^2)$.
\begin{enumerate}
\item For~$i = 1,2$, define $s_i = H(X_i/a)$.
\item Let~$n â‰¥ \abs{s_2-s_1} âˆš{a/(8Î´)}$.
\item Define the points~$(x_i=a H^{-1}(s_1 + \frac{i}{n}(s_2-s_1), f(x_i))$
as in Prop.~\ref{prop:points}.
\end{enumerate}
\end{prop}


\section{Arc length of an Archimedean spiral (wrapped line segment)}%Â«Â«1

Let~$F$ be the transformation on~$â„^2$ defined by
$F(x,y) = (x \cos(y/x), x \sin(y/x)$.

\begin{prop}
Let~$S = (p_0, p_1)$ be a line segment, with $p_i = (x_i, y_i)$,
such that $0 < x_0 < x_1$.
Let~$a = x_0 - x_1$, $D = x_0 y_1 - y_0 x_1$,
and $z_i = D+âˆš{a^2 x_i^2 + D^2}$.
Then the arc length of the image curve~$F(S)$ is
\[ \begin{cases}
  \frac{D}{a} \log \frac{x_1 z_0}{x_0 z_1}
	+ a \pa{\frac{x_1^2}{z_1}-\frac{x_0^2}{z_0}}&
	\text{if $x_0 â‰ Â x_1$;}\\
	x_0 \abs{y_0 - y_1} &\text{if $x_0 = x_1$.}\end{cases}
\]
\end{prop}
\begin{proof}
The segment is parametrized as $p(t) = (1-t) p_0 + p_1
 = (t (x_1-x_0) + x_0, t (y_1 - y_0) + y_0).
 = (a t +  b, c t + d)$
with $a = (x_1-x_0)$, $b = x_0$, $c = (y_1 - y_0)$, $d = y_0$.
In complex notation, one finds
$F(p(t)) = (a t + b) \exp(i \frac{ct+d}{at+b})$ and hence
\begin{eqsplit} F'(p(t))
&= a e^{iâ€¦} + (a t + b) i \frac{bc-ad}{(at+b)^2} e^{iâ€¦} \\
&= \pa{a + i \frac{bc - ad}{at + b}} \exp\pa{i \frac{ct+d}{at+b}};\\
\abs{F'(p(t))}
&= âˆš{a^2 + \frac{(ad-bc)^2}{(at+b)^2}}.
\end{eqsplit}
The arc length is therefore
\begin{eqsplit}
&= âˆ«_0^1 \abs{F'(p(t))} dt
&= âˆ«_0^1 âˆš{a^2 + \frac{(ad-bc)^2}{(at+b)^2}} dt\\
&= âˆ«_0^1 âˆš{a^2(at+b)^2 + (ad-bc)^2} \;\frac{dt}{at+b} \\
% &= a âˆ«_0^1 âˆš{(at+b)^2 + (d-bc/a)^2} \;\frac{dt}{at+b} \\
\end{eqsplit}
Define $s = (at+b)/(D+âˆš{a^2(at+b)^2+D^2})$,
so that $t = -b/a+2sD/(a^2(1-s^2))$,
$âˆš{(at+b)^2+D^2/a^2} = D\frac{1+s^2}{1-s^2}$,
and $dt = 2D/a^2 \frac{1+s^2}{(1-s^2)^2} ds$.
Then
\begin{eqsplit}
G(t) = âˆ« \abs{F'(p(t))} dt
&= \frac{D}{a} âˆ« \pa{\frac{1+s^2}{1-s^2}}^2 \frac{ds}{s}\\
&= \frac{D}{a} âˆ« \pa{\frac 1s +\frac{1}{(s-1)^2} - \frac{1}{(s+1)^2}} ds\\
&= \frac{D}{a} \pa{\log s + \frac{2}{1-s^2}}\\
&= \frac{D}{a} \pa{\log \frac{at+b}{D+âˆš{a^2(at+b)^2+D^2}}
 + 2 \frac{(D+âˆš{a^2(at+b)^2+D^2})^2}{(D+âˆš{a^2(at+b)^2+D^2})^2-(at+b)^2}}\\
&= \frac{D}{a} \pa{\log \frac{at+b}{D+âˆš{â€¦}}
 + 2 + \frac{a^2}{D}\frac{(at+b)^2}{D+âˆš{â€¦}}}\\
&= \frac{D}{a} \log \frac{at+b}{D+âˆš{a^2(at+b)^2+D^2}} + \frac{2D}{a}
 + a \frac{(at+b)^2}{D+âˆš{a^2(at+b)^2+D^2}}
\end{eqsplit}
The primitive~$G-2D/a$ takes the following values:
\begin{eqsplit}
G(0)
&= \frac{D}{a} \log \frac{x_0}{D+âˆš{a^2 x_0^2 + D^2}}
 + \frac{a x_0^2}{D+âˆš{a^2 x_0^2+D^2}}\\
G(1)
&= \frac{D}{a} \log \frac{x_1}{D+âˆš{a^2 x_1^2+D^2}}
 + \frac{a x_1^2}{D+âˆš{a^2 x_1^2+D^2}}\\
\end{eqsplit}
This concludes the case where~$a â‰ Â 0$. The other case is trivial.
\end{proof}

% &= âˆ«_0^1 âˆš{1+\frac{(ad-bc)^2}{a^2 (at+b)^2}}\; a dt\\
% % u = at + b; dt = 1/a du
% &= âˆ«_b^{a+b} âˆš{1+\frac{(ad-bc)^2}{a^2 u^2}}\; du\\
% &= âˆ«_{x_0}^{x_1} âˆš{1+k^2/u^2}\; du,
% \end{eqsplit}
% where~$k = (bc-ad)/a = \frac{x_0 y_1 - y_0 x_1}{x_1 - x_0}$.
% (Warning: if $x_0 = x_1$ then $k$ is infinite, we need asymptotics)
% 
% Let $v = u/(k+âˆš{u^2+k^2})$, so that
% $u = 2 k^2 v/(1-v^2)$, $âˆš{u^2+k^2} = k(1+v^2)/(1-v^2)$
% and $du = 2k(1+v^2)/(1-v^2)^2$. Then
% \begin{eqsplit}
% âˆ« âˆš{k^2+u^2} du/u
% &= âˆ« \pa{\frac{1+v^2}{1-v^2}}^2 \frac{k\, dv}{v} \\
% &= k âˆ« \pa{1
% +\frac{1}{v-1}-\frac{1}{v+1}+\frac{1}{(v-1)^2}+\frac{1}{(v+1)^2}} dv \\
% &= k (v + \log(1-v) - \log(v+1) +\frac{1}{1-v} -\frac{1}{1+v}) \\
% &= k (v + \log\frac{1-v}{1+v} + \frac{2v}{1-v^2}) \\
% &= \frac{k u}{k+âˆš{u^2+k^2}} + k \log\frac{k-u+âˆš{k^2+u^2}}{k+u+âˆš{k^2+u^2}} + u \\
% \end{eqsplit}
\end{document}
